Completeness

theories/Completeness.v
@@ -41,27 +41,96 @@ From Must Require Import Lift.
 Class gen_spec {P A : Type} `{Lts P A, !LtsEq P A, !Good P A good}
   (co_of : A -> A) (gen : list A -> P) := {
             co_inter μ : parallel_inter μ (co_of μ);
-                (* co_of μ interragît avec μ *)
+                (* co_of μ interract with μ *)
             co_inter_spec1 μ μ': 
                 parallel_inter μ' (co_of μ)
                           -> μ = μ';
-                (* co_of μ n'interragît qu'avec μ *)
+                (* co_of μ interract only with μ *)
     (* 1 *) gen_spec_ungood : 
               forall s, ¬ good (gen s) ;
     (* 2 *) gen_spec_mu_lts_co μ1 (* μ2 *) s :
               gen (μ1 :: s) ⟶⋍[co_of μ1] gen s;
-    (* 3 *) gen_spec_out_lts_tau_ex μ s : 
-              (* non_blocking μ ->  *) 
+    (* 3 *) gen_spec_co_not_nb_lts_tau_ex μ s : 
+              (* non_blocking μ ->  *)
+              ¬ non_blocking (co_of μ) ->
               ∃ e', gen (μ :: s) ⟶ e';
-    (* 4 *) gen_spec_out_lts_tau_good η s e : 
-              (* non_blocking η -> *) 
-              gen (η :: s) ⟶ e -> good e;
-    (* 5 *) gen_spec_out_lts_mu_uniq {e η μ s} : (* unique ???? *)
+    (* 4 *) gen_spec_co_not_nb_lts_tau_good μ s e : 
+              (* non_blocking η -> *)
+              ¬ non_blocking (co_of μ) ->
+              gen (μ :: s) ⟶ e -> good e;
+    (* 5 *) gen_spec_co_not_nb_lts_mu_uniq {e μ μ' s} : (* unique ???? *)
               (* non_blocking η ->  *)
-              ¬ non_blocking μ ->
-              gen (η :: s) ⟶[μ] e -> e ⋍ gen s /\ μ = co_of η;
+              ¬ non_blocking (co_of μ) ->
+              gen (μ :: s) ⟶[μ'] e -> e ⋍ gen s /\ μ' = co_of μ;
   }.
+
+Lemma co_of_inj `{
+  M1 : LtsOba E A, !Good E A good, !gen_spec co_of f}
+  μ μ' :
+  co_of μ = co_of μ' -> μ = μ'.
+Proof.
+  intro eq. 
+  assert (parallel_inter μ' (co_of μ)) as inter. rewrite eq.
+  eapply co_inter. eapply co_inter_spec1. exact inter.
+Qed.
+
+Lemma co_co_is_id `{
+  M1 : LtsOba E A, !Good E A good, !gen_spec co_of f} 
+  μ :
+  μ = co_of (co_of μ).
+Proof.
+  assert (parallel_inter (co_of (co_of μ)) (co_of μ)) as inter.
+  symmetry. eapply co_inter.
+  eapply co_inter_spec1. exact inter.
+Qed.
+
+
+Lemma co_is_co_of_nb `{
+  M1 : LtsOba E A, !Good E A good, !gen_spec co_of f} 
+  μ :
+  non_blocking (co_of μ) -> co_of μ = co μ.
+Proof.
+  intro nb. assert (parallel_inter μ (co_of μ)) as inter.
+  eapply co_inter. 
+  eapply unique_nb; eauto.
+Qed.
+
+(* à voir*)
+(* Lemma co_of_is_co_nb' `{
+  M1 : LtsOba E A, !Good E A good, !gen_spec co_of f} 
+  μ :
+  non_blocking (co μ) (* -> dual (co μ) μ *) -> co_of μ = co μ.
+Proof.
+  intros nb. (* duo. *)
+  assert (parallel_inter μ (co_of μ)) as inter. eapply co_inter.
+  assert (¬ non_blocking μ) as not_nb. eapply lts_oba_fw_non_blocking_duo_spec in nb ; eauto.
   
+  assert (exists μ', dual (co μ) μ'). eapply exists_duo_nb; eauto.
+  destruct H0 as (x & duo).
+  
+  assert ((co μ) = co x). eapply unique_nb; eauto. subst.
+  
+  
+  eapply unique_nb; eauto.
+  assert (¬ non_blocking (co_of (co μ))) as not_nb'.
+  eapply lts_oba_fw_non_blocking_duo_spec in nb ; eauto. symmetry. eapply co_inter.
+  eapply nb_not_nb; eauto.
+Qed. *)
+
+Lemma co_of_is_co_nb `{
+  M1 : LtsOba E A, !Good E A good, !gen_spec co_of f} 
+  μ :
+  non_blocking (co μ) -> dual (co μ) μ -> co_of μ = co μ.
+Proof.
+  intros nb duo.
+  assert (parallel_inter μ (co_of μ)) as inter. eapply co_inter.
+  assert (¬ non_blocking μ) as not_nb. eapply lts_oba_fw_non_blocking_duo_spec in nb ; eauto.
+  eapply unique_nb; eauto.
+  assert (¬ non_blocking (co_of (co μ))) as not_nb'.
+  eapply lts_oba_fw_non_blocking_duo_spec in nb ; eauto. symmetry. eapply co_inter.
+  eapply nb_not_nb; eauto.
+Qed. 
+
 Lemma gen_spec_determinacy `{
   M1 : LtsOba E A, !Good E A good, !gen_spec co_of f} 
   μ1 s e:
@@ -72,7 +141,7 @@ Proof.
   + assert (f (μ1 :: s) ⟶⋍[co_of μ1] f s) as (e' & Tr & Eq). eapply gen_spec_mu_lts_co.
     assert (e' ⋍ e) as equiv. eapply lts_oba_non_blocking_action_deter; eauto.
     etransitivity; eauto. symmetry; eauto.
-  + eapply gen_spec_out_lts_mu_uniq in not_nb as (equi & Tr); eauto.
+  + eapply gen_spec_co_not_nb_lts_mu_uniq in not_nb as (equi & Tr); eauto.
 Qed.
 
 
@@ -92,15 +161,15 @@ Class gen_spec_acc {P : Type} `{Lts P A, ! LtsEq P A, !Good P A good}
     gen_acc_spec_gen_spec O : gen_spec co_of (gen_acc O) ;
     (* t1 *) gen_spec_acc_nil_stable_tau O : 
                 gen_acc O [] ↛ ;
-    (* t2 *) gen_spec_acc_nil_stable_out O η : 
+    (* t2 *) gen_spec_acc_nil_stable_nb O η : 
                 non_blocking η -> gen_acc O [] ↛[η] ;
   (* t3-> *) gen_spec_acc_nil_mu_inv O μ e : 
                 ¬ non_blocking μ -> gen_acc O [] ⟶[μ] e
                     -> (exists η, μ = co_of η /\ O η) ;
   (* t3<- *) gen_spec_acc_nil_mem_lts_inp O η : 
                 O η (* η ∈ O *) -> ∃ r μ, gen_acc O [] ⟶[μ] r /\ μ = co_of η;
-    (* t4 *) gen_spec_acc_nil_lts_inp_good μ e' O : 
-                gen_acc O [] ⟶[μ] e' -> good e' ;
+    (* t4 *) gen_spec_acc_nil_lts_not_nb_good μ e' O : 
+                ¬ non_blocking μ -> gen_acc O [] ⟶[μ] e' -> good e' ;
   }.
 
 #[global] Existing Instance gen_acc_spec_gen_spec.
@@ -147,7 +216,13 @@ Lemma gen_conv_always_reduces `{
 Proof.
   induction s as [|μ s'].
   - eapply gen_spec_conv_nil_lts_tau_ex.
-  - eapply gen_spec_out_lts_tau_ex.
+  - destruct (decide (non_blocking (co_of μ))) as [nb | not_nb]. 
+    + destruct IHs' as (e & l).
+      destruct (gen_spec_mu_lts_co μ s') as (e' & hl' & heq).
+      destruct (eq_spec e' e τ) as (e0 & hl0 & heqe0). eauto with mdb.
+      destruct (lts_oba_non_blocking_action_delay nb hl' hl0)
+        as (r & l1 & l2); eauto.
+    + eapply gen_spec_co_not_nb_lts_tau_ex. exact not_nb.
 Qed.
 
 Lemma terminate_must_test_conv_nil `{
@@ -255,7 +330,7 @@ Proof.
       etransitivity. symmetry. exact equiv. etransitivity; eauto.
     + destruct HypTr as (e & HypTr & equiv).
       assert (e ⋍ f s2 /\ co_of μ = co_of μ) as (equiv' & eq'). 
-      eapply gen_spec_out_lts_mu_uniq; eauto.
+      eapply gen_spec_co_not_nb_lts_mu_uniq; eauto.
       etransitivity. symmetry. exact equiv. eauto.
   - inversion his; subst.
     destruct (decide (non_blocking (co_of μ))) as [nb | not_nb].
@@ -263,21 +338,33 @@ Proof.
       eapply f_gen_lts_mu_in_the_middle. eauto.
       destruct HypTr as (e & HypTr & equiv).
       destruct HypTr' as (e' & HypTr' & equiv').
-      simpl in *. assert (e ⋍ e').
+      assert (e ⋍ e').
       eapply lts_oba_non_blocking_action_deter; eauto. 
       etransitivity. symmetry. exact equiv. etransitivity; eauto.
     + destruct HypTr as (e & HypTr & equiv).
-      assert (e ⋍ f (s' ++ μ :: s2) /\ co_of μ = co_of ν) as (equiv' & eq'). 
-      eapply gen_spec_out_lts_mu_uniq; eauto. 
-      
-      assert (μ = ν). eapply co_inter_spec1. rewrite eq'. eapply co_inter.
-      subst.
-      
-      
-      destruct H3 as (ν' & nb & duo).
-      
-      assert (non_blocking (co_of ν)). eapply nb_not_nb; eauto. eapply co_inter.
-      contradiction.
+      destruct (decide (non_blocking (co_of ν))) as [nb' | not_nb'].
+      ++ assert (f (ν :: s' ++ μ :: s2) ⟶⋍[co_of ν] f (s' ++ μ :: s2)) as HypTr'.
+         eapply gen_spec_mu_lts_co. destruct HypTr' as (e' & HypTr' & equiv').
+         assert (co_of μ <> co_of ν) as not_eq. intro imp. rewrite imp in not_nb. contradiction.
+         destruct (lts_oba_non_blocking_action_confluence nb' not_eq HypTr' HypTr )
+           as (t' & l2 & (t & l1 & heq)).
+         assert (f (s' ++ μ :: s2) ⟶⋍[co_of μ] f (s' ++ s2)) as HypTr''.
+         eapply f_gen_lts_mu_in_the_middle; eauto.
+         edestruct (eq_spec (f (s' ++ μ :: s2)) t' (ActExt (co_of μ)))
+          as (v & hlv & heqv).
+         exists e'. split; eauto. symmetry; eauto.
+         assert (t' ⋍ (f (s' ++ s2))) as heq'. eapply IHs'; eauto.
+         exists v. split; eauto.
+         assert (f (ν :: s' ++ s2) ⟶⋍[co_of ν] f (s' ++ s2)) as (v' & hlv' & heqv').
+         eapply gen_spec_mu_lts_co.
+         assert (e ⋍ f (ν :: s' ++ s2)) as final. 
+         eapply lts_oba_non_blocking_action_deter_inv; eauto.
+         etransitivity. exact heq. etransitivity. exact heq'. symmetry; eauto.
+         etransitivity. symmetry. exact equiv. eauto.
+      ++ destruct H3 as (ν' & nb & duo).
+         assert (parallel_inter ν (co_of ν)). eapply co_inter.
+         assert (non_blocking (co_of ν)).
+         eapply nb_not_nb; eauto. contradiction.
 Qed.
 
 Lemma inversion_gen_mu_not_nb `{
@@ -287,7 +374,8 @@ Lemma inversion_gen_mu_not_nb `{
   f s ⟶[μ'] p ->
   ¬ non_blocking μ' -> 
   ¬ good p ->
-  ∃ s1 s2 μ, s = s1 ++ μ :: s2 /\ p ⋍ f (s1 ++ s2) /\ μ' = co_of μ /\ Forall exist_co_nba s1.
+  ∃  s1 s2 μ, s = s1 ++ μ :: s2 /\ p ⋍ f (s1 ++ s2) 
+  /\ μ' = co_of μ  /\ Forall exist_co_nba s1 (* /\ (¬ non_blocking μ' -> s1 = []) *).
 Proof.
   revert μ' p.
   induction s
@@ -297,8 +385,29 @@ Proof.
   - edestruct (h μ) as [stable_f | f_to_good].
     + now eapply lts_stable_spec2 in stable_f; eauto.
     + assert (good p). eapply f_to_good. eauto. contradiction.
-  - destruct (gen_spec_out_lts_mu_uniq not_nb l); subst.
-    exists [], s', ν. simpl. repeat split; simpl; eauto with mdb.
+  - destruct (decide (non_blocking (co_of ν))) as [nb' | not_nb'].
+    + assert (f (ν :: s') ⟶⋍[co_of ν] f s') as (v & hlv & eqv).
+      eapply gen_spec_mu_lts_co. assert (μ <> (co_of ν)) as not_eq.
+      eapply BlockingAction_are_not_non_blocking; eauto.
+      destruct (lts_oba_non_blocking_action_confluence nb' not_eq hlv l)
+           as (t' & l2 & (t & l1 & heq)).
+      destruct (eq_spec (f s') t' (ActExt μ)) as (v' & hlv' & heqv').
+      exists v. split. symmetry; eauto. exact l2.
+      destruct (decide (good v')) as [happy' | not_happy'].
+      ++ exfalso. assert (good p).
+         eapply good_preserved_by_lts_non_blocking_action_converse; eauto.
+         eapply good_preserved_by_eq; eauto. etransitivity; eauto. symmetry. eauto.
+         contradiction.
+      ++ edestruct (Hlength s') as (s1 & s2 & μ' & eq1 & eq2 & equiv' & eq3 (*& eq4*)); eauto. 
+         subst.
+         assert (p ⋍ f ((ν :: s1) ++ s2)). eapply f_gen_lts_mu_in_the_middle'.
+         constructor; eauto. exists (co_of ν). split; eauto. eapply co_inter. simpl.
+         exists p. split; eauto. reflexivity.
+         exists (ν :: s1). exists s2. exists μ'.
+         split. eauto. split; eauto. split; eauto.
+         constructor; eauto. exists (co_of ν). split; eauto. eapply co_inter.
+    + destruct (gen_spec_co_not_nb_lts_mu_uniq not_nb' l); subst.
+      exists [], s', ν. simpl. repeat split; simpl; eauto with mdb.
 Qed.
 
 
@@ -309,7 +418,8 @@ Lemma inversion_gen_mu_nb `{
   f s ⟶[μ] p ->
   non_blocking μ -> 
   ¬ good p ->
-  ∃ s1 s2 μ', s = s1 ++ μ' :: s2 /\ p ⋍ f (s1 ++ s2) /\ μ = co_of μ' /\ Forall exist_co_nba s1.
+  ∃ s1 s2 μ', s = s1 ++ μ' :: s2 /\ p ⋍ f (s1 ++ s2) /\ μ = co_of μ' 
+    /\ Forall exist_co_nba s1 (* /\ (¬ non_blocking μ -> s1 = []) *).
 Proof.
   revert μ p.
   induction s
@@ -333,7 +443,7 @@ Proof.
              eapply good_preserved_by_lts_non_blocking_action_converse; eauto.
              assert (¬ good (f s')). eapply gen_spec_ungood. contradiction.
          +++ edestruct (Hlength s' ltac:(eauto) μ v h hlv nb not_happy')
-             as (s1' & s2' & μ' & eq0 & eq1 & eq2 & eq3); eauto. subst.
+             as (s1' & s2' & μ' & eq0 & eq1 & eq2 & eq3 (* & eq4 *)); eauto. subst.
              destruct (decide (non_blocking (co_of ν))) as [nb' | not_nb'].
              ++++ assert (¬ non_blocking ν) as not_nb''.
                   eapply lts_oba_fw_non_blocking_duo_spec; eauto. eapply co_inter.
@@ -352,241 +462,57 @@ Proof.
                   transitivity t. symmetry. eassumption.
                   transitivity v. now symmetry.
                   transitivity (f (s1' ++ s2')). eassumption. now symmetry.
-            ++++ assert (¬ non_blocking μ') as not_nb''.
-                 eapply lts_oba_fw_non_blocking_duo_spec; eauto. eapply co_inter.
-                 
-                 assert (r ⋍ f (s1' ++ μ' :: s2')) as equiv. eapply gen_spec_determinacy; eauto.
-                 
-                 assert (¬ good r) as not_happy''. assert (¬ good (f (s1' ++ μ' :: s2'))) as not_happy'''.
-                 eapply gen_spec_ungood. eapply ungood_preserved_by_eq; eauto. 
-                 
-                 assert (f (ν :: s1' ++ μ' :: s2') ⟶[co_of ν] r) as HypTr; eauto.
-                 eapply (inversion_gen_mu_not_nb (ν :: s1' ++ μ' :: s2') (co_of ν) r) in HypTr ; eauto.
-                 
-                 destruct HypTr.
+                  (* intro not_nb'''. contradiction. *)
+            ++++ assert (p ⋍ f (s1' ++ μ' :: s2') /\ co_of μ' = co_of ν) as (equiv''' & eq''').
+                 eapply gen_spec_co_not_nb_lts_mu_uniq; eauto.
+                 assert (μ' = ν). eapply co_of_inj. eauto. subst. contradiction.
+Qed.
 
-Admitted.
-
-
-(* Lemma inversion_gen_mu `{
+Lemma inversion_gen_mu `{
   M1 : LtsOba E A, !Good E A good, !gen_spec co_of f} 
-  s μ' p :
+  s μ p :
   (forall μ, f [] ↛[μ] \/ (forall e, f [] ⟶[μ] e -> good e)) ->
-  f s ⟶[μ'] p ->
-  non_blocking μ' -> 
+  f s ⟶[μ] p ->
   ¬ good p ->
-  ∃ s1 s2 μ, s = s1 ++ μ :: s2 /\ p ⋍ f (s1 ++ s2) /\ μ' = co_of μ /\ Forall exist_co_nba s1.
+  ∃ s1 s2 μ', s = s1 ++ μ' :: s2 /\ p ⋍ f (s1 ++ s2) 
+    /\ μ = co_of μ' /\ Forall exist_co_nba s1 .
 Proof.
-  revert μ' p.
-  induction s
-    as (s & Hlength) using
-         (well_founded_induction (wf_inverse_image _ nat _ length Nat.lt_wf_0)).
-  destruct s as [|ν s']; intros μ p h l nb not_happy.
-  - edestruct (h μ) as [stable_f | f_to_good].
-    + now eapply lts_stable_spec2 in stable_f; eauto.
-    + exfalso. eapply not_happy. eapply f_to_good; eauto.
-  - edestruct (gen_spec_mu_lts_co ν s') as (r & hlr & heqr).
-      destruct (decide (co_of ν = μ)) as [eq | neq].
-      ++ subst.
-         exists [], s', ν. repeat split; simpl; eauto with mdb.
-         transitivity r; eauto. 
-         eapply (lts_oba_non_blocking_action_deter nb l hlr); eauto.
-      ++ destruct (lts_oba_non_blocking_action_confluence nb neq l hlr )
-           as (p' & l2 & r' & l1 & heq).
-         destruct (eq_spec (f s') r' (ActExt $ μ)) as (v & hlv & heqv).
-         exists r. split; eauto with mdb. now symmetry.
-         destruct (decide (good v)) as [happy' | not_happy'].
-         +++ exfalso. assert (good (f s')). 
-             eapply good_preserved_by_lts_non_blocking_action_converse; eauto.
-             assert (¬ good (f s')). eapply gen_spec_ungood. contradiction.
-         +++ edestruct (Hlength s' ltac:(eauto) μ v h hlv nb not_happy')
-             as (s1' & s2' & μ' & eq0 & eq1 & eq2 & eq3); eauto.
-             
-             
-              
-             assert (r ⋍ f(s')) as equiv'. eapply gen_spec_determinacy; eauto.
-             symmetry in equiv'. edestruct (eq_spec (f s') r') as (r'' & HypTr'' & equiv''). 
-             exists r; eauto. subst.
-             assert (¬ non_blocking μ') as not_nb. 
-             eapply lts_oba_fw_non_blocking_duo_spec; eauto. eapply co_inter.
-             assert (Forall exist_co_nba (μ' :: s1')).
-             constructor. exists (co_of μ'). split; eauto. eapply co_inter. eauto.
-             exists (ν :: s1'). exists s2'. exists μ'.
-             split. eauto. 
-             split. 
-             destruct (decide (non_blocking ν)) as [nb' | not_nb'].
-             + admit.
-             + eapply inversion_gen_mu_nb in hlr.
-             
-              
-             
-             
-         right.
-         exists [], s', ν.
-         repeat split; eauto. simpl.
-                  
-         +++ (*right. exists (ActIn b :: s1'), s2'. repeat split; eauto.
-             destruct μ; subst; eauto.
-             edestruct (f_gen_lts_mu_in_the_middle (ActIn b :: s1') s2' (ActIn b))
-               as (r' & hlr' & heqr').
-             eapply Forall_cons. split; eauto. eexists. reflexivity.
-             edestruct (gen_spec_mu_lts_co (ActIn b) (s1' ++ s2'))
-               as (w & hlw & heqw).
-             eapply lts_oba_output_deter_inv; try eassumption.
-             transitivity t. eassumption.
-             transitivity v. now symmetry.
-             transitivity (f (s1' ++ s2')). eassumption. now symmetry.
-             eapply Forall_cons. split; eauto. eexists. reflexivity. *) admit.
+  intros. destruct (decide (non_blocking μ)) as [nb | not_nb].
+  + eapply inversion_gen_mu_nb; eauto.
+  + eapply inversion_gen_mu_not_nb; eauto.
 Qed.
 
-  
-  
-  
-  
-  destruct (decide (non_blocking μ)) as [nb | not_nb].
-    + edestruct (gen_spec_mu_lts_co ν s') as (r & hlr & heqr).
-      destruct (decide (non_blocking (co_of ν))) as [nb' | not_nb'].
-      ++ subst.
-         right. exists [], s', ν. repeat split; simpl; eauto with mdb.
-         transitivity r; eauto. admit. 
-         (* eapply (lts_oba_non_blocking_action_deter nb l hlr); eauto. *)
-         (* +++ destruct (decide (non_blocking (co_of ν))) as [nb' | not_nb'].
-             ++++ left.
-                  eapply good_preserved_by_lts_non_blocking_action_converse. exact nb'.
-                  exact l2. eapply good_preserved_by_eq; eauto.
-                  transitivity r' ; now symmetry. *)
-      ++ assert (co_of ν ≠ μ) as neq. eapply BlockingAction_are_not_non_blocking; eauto.
-         destruct (lts_oba_non_blocking_action_confluence nb neq l hlr )
-           as (p' & l2 & r' & l1 & heq).
-         destruct (eq_spec (f s') r' (ActExt $ μ)) as (v & hlv & heqv).
-         exists r. split; eauto with mdb. now symmetry.
-         edestruct (Hlength s' ltac:(eauto) μ v h hlv)
-           as [hg | (s1' & s2' & eq0 & eq1 & eq2)]; eauto.
-         right.
-                  exists [], s', ν.
-                  repeat split; eauto. simpl.
-                  
-         +++ (*right. exists (ActIn b :: s1'), s2'. repeat split; eauto.
-             destruct μ; subst; eauto.
-             edestruct (f_gen_lts_mu_in_the_middle (ActIn b :: s1') s2' (ActIn b))
-               as (r' & hlr' & heqr').
-             eapply Forall_cons. split; eauto. eexists. reflexivity.
-             edestruct (gen_spec_mu_lts_co (ActIn b) (s1' ++ s2'))
-               as (w & hlw & heqw).
-             eapply lts_oba_output_deter_inv; try eassumption.
-             transitivity t. eassumption.
-             transitivity v. now symmetry.
-             transitivity (f (s1' ++ s2')). eassumption. now symmetry.
-             eapply Forall_cons. split; eauto. eexists. reflexivity. *) admit.
-    + right.
-      destruct (gen_spec_out_lts_mu_uniq not_nb l); subst.
-      exists [], s', ν. simpl. repeat split; simpl; eauto with mdb.
-
-
-
-
-
-
-
-
-
-
-
-
-
-  revert μ' p.
-  induction s
-    as (s & Hlength) using
-         (well_founded_induction (wf_inverse_image _ nat _ length Nat.lt_wf_0)).
-  destruct s as [|ν s']; intros μ p h l.
-  - edestruct (h μ) as [stable_f | f_to_good].
-    + now eapply lts_stable_spec2 in stable_f; eauto.
-    + eauto.
-  - destruct (decide (non_blocking μ)) as [nb | not_nb].
-    + edestruct (gen_spec_mu_lts_co ν s') as (r & hlr & heqr).
-      destruct (decide (non_blocking (co_of ν))) as [nb' | not_nb'].
-      ++ subst.
-         right. exists [], s', ν. repeat split; simpl; eauto with mdb.
-         transitivity r; eauto. admit. 
-         (* eapply (lts_oba_non_blocking_action_deter nb l hlr); eauto. *)
-         (* +++ destruct (decide (non_blocking (co_of ν))) as [nb' | not_nb'].
-             ++++ left.
-                  eapply good_preserved_by_lts_non_blocking_action_converse. exact nb'.
-                  exact l2. eapply good_preserved_by_eq; eauto.
-                  transitivity r' ; now symmetry. *)
-      ++ assert (co_of ν ≠ μ) as neq. eapply BlockingAction_are_not_non_blocking; eauto.
-         destruct (lts_oba_non_blocking_action_confluence nb neq l hlr )
-           as (p' & l2 & r' & l1 & heq).
-         destruct (eq_spec (f s') r' (ActExt $ μ)) as (v & hlv & heqv).
-         exists r. split; eauto with mdb. now symmetry.
-         edestruct (Hlength s' ltac:(eauto) μ v h hlv)
-           as [hg | (s1' & s2' & eq0 & eq1 & eq2)]; eauto.
-         right.
-                  exists [], s', ν.
-                  repeat split; eauto. simpl.
-                  
-         +++ (*right. exists (ActIn b :: s1'), s2'. repeat split; eauto.
-             destruct μ; subst; eauto.
-             edestruct (f_gen_lts_mu_in_the_middle (ActIn b :: s1') s2' (ActIn b))
-               as (r' & hlr' & heqr').
-             eapply Forall_cons. split; eauto. eexists. reflexivity.
-             edestruct (gen_spec_mu_lts_co (ActIn b) (s1' ++ s2'))
-               as (w & hlw & heqw).
-             eapply lts_oba_output_deter_inv; try eassumption.
-             transitivity t. eassumption.
-             transitivity v. now symmetry.
-             transitivity (f (s1' ++ s2')). eassumption. now symmetry.
-             eapply Forall_cons. split; eauto. eexists. reflexivity. *) admit.
-    + right.
-      destruct (gen_spec_out_lts_mu_uniq not_nb l); subst.
-      exists [], s', ν. simpl. repeat split; simpl; eauto with mdb.
-
-
-  - right. destruct (decide (non_blocking μ)) as [nb | not_nb].
-    + (* exists ν, s'. repeat split; simpl; eauto with mdb.*) admit.
-    + destruct (gen_spec_out_lts_mu_uniq not_nb l) as (equiv & eq); subst.
-      exists ν, s'. repeat split; simpl; eauto with mdb.
-      eapply co_inter.
-Qed.
- *)
 Lemma inversion_gen_mu_gen_conv `{
   M1 : LtsOba E A, !Good E A good, !gen_spec_conv co_of f}
   s μ p :
   f s ⟶[μ] p ->
   good p \/ 
-  ∃ s1 s2 μ', s = s1 ++ μ' :: s2 /\ p ⋍ f (s1 ++ s2) /\ μ = co_of μ' /\ Forall exist_co_nba s1.
+  ∃ s1 s2 μ', s = s1 ++ μ' :: s2 /\ p ⋍ f (s1 ++ s2) /\ μ = co_of μ' 
+    /\ Forall exist_co_nba s1 .
 Proof.
   intros. 
   destruct (decide (good p)) as [happy | not_happy].
   + left; eauto.
-  + right. 
-    destruct (decide (non_blocking μ)) as [nb | not_nb]. 
-    ++ eapply inversion_gen_mu_nb; eauto.
-       intros. left. eapply gen_spec_conv_nil_stable_mu; eauto.
-    ++ eapply inversion_gen_mu_not_nb; eauto.
-       intros. left. eapply gen_spec_conv_nil_stable_mu; eauto.
+  + right. eapply inversion_gen_mu; eauto.
+    intros. left. eapply gen_spec_conv_nil_stable_mu; eauto.
 Qed.
 
-Lemma inversion_gen_mu_gen`{
+Lemma inversion_gen_mu_gen_acc`{
   M1 : LtsOba E A, !Good E A good, !gen_spec_acc co_of f} 
   s μ p O :
   f O s ⟶[μ] p ->
   good p \/ 
-  ∃ s1 s2 μ', s = s1 ++ μ' :: s2 /\ p ⋍ f O (s1 ++ s2) /\ μ = co_of μ' /\ Forall exist_co_nba s1.
+  ∃ s1 s2 μ', s = s1 ++ μ' :: s2 /\ p ⋍ f O (s1 ++ s2) /\ μ = co_of μ' 
+  /\ Forall exist_co_nba s1 .
 Proof.
   intros. 
   destruct (decide (good p)) as [happy | not_happy].
   + left; eauto.
-  + right. 
-    destruct (decide (non_blocking μ)) as [nb | not_nb]. 
-    ++ eapply inversion_gen_mu_nb; eauto.
-       intros. left. eapply gen_spec_conv_nil_stable_mu; eauto.
-    ++ eapply inversion_gen_mu_not_nb; eauto.
-       intros. left. eapply gen_spec_conv_nil_stable_mu.
-       
-    Unshelve. eauto.
-     eauto.  eauto. eauto. eauto. eauto. eauto. eauto. eauto. eauto. eauto. eauto.
-
+  + right. eapply inversion_gen_mu; eauto. intro μ'.
+    destruct (decide (non_blocking μ')) as [nb' | not_nb'].
+       +++ left. eapply gen_spec_acc_nil_stable_nb. exact nb'.
+       +++ right. intro HypTr. eapply gen_spec_acc_nil_lts_not_nb_good. exact not_nb'.
+Qed.
 
 Definition not_non_blocking `{ExtAction A} μ := ¬ non_blocking μ.
 
@@ -596,27 +522,95 @@ Lemma inversion_gen_tau `{
   (f [] ↛ \/ (forall e, f [] ⟶ e -> good e)) ->
   (forall μ, f [] ↛[μ] \/ (forall e, f [] ⟶[μ] e -> good e)) ->
   f s ⟶ q ->
-  good q. (* \/ (∃ μ μ' (s1 : list A) s2 s3, s = s1 ++ [μ] ++ s2 ++ [μ'] ++ s3
-                          /\ parallel_inter μ μ'
+  good q \/ (∃ μ s1 s2 s3, s = s1 ++ [μ] ++ s2 ++ [co_of μ] ++ s3
                           /\ q ⋍ f (s1 ++ s2 ++ s3)
-                          /\ ¬ non_blocking μ
-                          /\ Forall (not_non_blocking) s1 
-                          /\ Forall (not_non_blocking) s2). *)
+                          /\ exist_co_nba μ
+                          /\ Forall exist_co_nba s1 
+                          /\ Forall exist_co_nba s2).
 Proof.
-  revert q. induction s as [|μ s']; intros q h1 h2 l.
+  revert q. induction s as [|μ' s']; intros q h1 h2 HypTr.
   - destruct h1 as [stable_f | f_to_good].
     + eauto. now eapply lts_stable_spec2 in stable_f ; eauto.
     + eauto. 
-  - eapply gen_spec_out_lts_tau_good; eauto.
+  - destruct (decide (non_blocking (co_of μ'))) as [nb | not_nb].
+    + destruct (decide (good q)) as [happy | not_happy].
+      ++ left. exact happy.
+      ++ assert (parallel_inter μ' (co_of μ')) as inter.
+         eapply co_inter.
+         assert (¬ non_blocking μ') as not_nb.
+         eapply lts_oba_fw_non_blocking_duo_spec; eauto.
+         edestruct (gen_spec_mu_lts_co μ' s') as (r & hlr & heqr).
+         destruct (lts_oba_non_blocking_action_tau nb hlr HypTr)
+         as [(r1 & l1 & (r2 & l2 & heq))| HypTr''].
+         +++ destruct (eq_spec (f s') r1 τ) as (v & hlv & heqv).
+             exists r. split; eauto with mdb. now symmetry.
+             destruct (IHs' _ h1 h2 hlv) as [happy' | Hyp].
+             ++++ exfalso. 
+                  assert (¬ good r2) as not_happy''.
+                  eapply ungood_preserved_by_lts_non_blocking_action; eauto.
+                  assert (¬ good v) as not_happy'.
+                  eapply ungood_preserved_by_eq; eauto.
+                  etrans. eapply heqv. now symmetry. 
+                  contradiction.
+             ++++ right.
+                  destruct Hyp as (μ & s1 & s2 & s3 & eq0 & eq1 & hi & his1 & his2).
+                  subst.
+                  exists μ, (μ' :: s1), s2, s3. cbn.
+                  repeat split; eauto.
+                  +++++ edestruct (gen_spec_mu_lts_co μ') as (w & hlw & heqw).
+                        eapply lts_oba_non_blocking_action_deter_inv. eassumption.
+                        eassumption. eassumption.
+                        etrans. eassumption.
+                        etrans. symmetry. eapply heqv.
+                        etrans. eassumption.
+                        now symmetry.
+                  +++++ eapply Forall_cons; split; eauto. exists (co_of μ'). split.
+                        exact nb. eapply co_inter.
+         +++ destruct HypTr'' as (μ & duo & HypTr').
+             assert (μ' = μ) as eq. eapply co_inter_spec1. exact duo.
+             subst.
+             assert (neq : μ <> co_of μ). intro eq_imp. rewrite eq_imp in not_nb.
+             contradiction.
+             destruct HypTr' as (q' & l' & heq).
+             edestruct (lts_oba_non_blocking_action_delay nb hlr l')
+           as (v & hlv & (t & l4 & heq4)).
+             edestruct (lts_oba_non_blocking_action_confluence nb neq hlr hlv)
+           as (r' & l3 & (t' & l4' & heq4')).
+             destruct (eq_spec (f s') r' (ActExt $ μ)) as (t0 & hlt0 & heqt0).
+             exists r. split. now symmetry. eassumption.
+             destruct (inversion_gen_mu _ _ _ h2 hlt0)
+           as (s1 & s2 & μ' & eq1 & eq2 & eq & his (* & eq3 *)). 
+             ++++ assert (t0 ⋍ q) as equiv.
+                  etrans. eauto.
+                  transitivity t'. now symmetry.
+                  symmetry. transitivity t.
+                  transitivity q'; now symmetry.
+                  eapply lts_oba_non_blocking_action_deter; eauto.
+                  eapply ungood_preserved_by_eq. eassumption. exact equiv.
+             ++++ subst.
+                  assert (μ' = co_of (co_of μ')) as eq. eapply co_co_is_id.
+                  right. exists (co_of μ'), [], s1, s2. repeat split; simpl; subst; eauto.
+                  +++++ symmetry. symmetry in eq. rewrite eq at 1. eauto.
+                  +++++ etrans. symmetry. eassumption.
+                        etrans. symmetry. eassumption.
+                        symmetry.
+                        etrans. symmetry. eassumption.
+                        etrans. eapply heqt0.
+                        etrans. symmetry. eapply heq4'.
+                        eapply lts_oba_non_blocking_action_deter; eassumption.
+                  +++++ exists (co_of (co_of μ')). split; eauto.
+    + left. eapply gen_spec_co_not_nb_lts_tau_good. exact not_nb. exact HypTr.
 Qed.
 
 Lemma inversion_gen_tau_gen_conv `{
   M1 : LtsOba E A, !Good E A good, !gen_spec_conv co_of f} 
   s q :
   f s ⟶ q ->
-  good q (* \/ (∃ μ s1 s2 s3, s = s1 ++ [μ] ++ s2 ++ [co μ] ++ s3
+  good q \/ (∃ μ s1 s2 s3, s = s1 ++ [μ] ++ s2 ++ [co_of μ] ++ s3
                           /\ q ⋍ f (s1 ++ s2 ++ s3)
-                          /\ is_input μ /\ are_inputs s1 /\ are_inputs s2) *).
+                          /\ exist_co_nba μ
+                          /\ Forall exist_co_nba s1 
+                          /\ Forall exist_co_nba s2).
 Proof.
   intros.
   eapply inversion_gen_tau; eauto.
@@ -624,19 +618,24 @@ Proof.
   intro μ. left. eapply gen_spec_conv_nil_stable_mu.
 Qed.
 
-(* Lemma inversion_gen_tau_gen_acc
-  `{M1 : LtsOba A L, !Good A L good, !gen_spec_acc f} s O q :
+Lemma inversion_gen_tau_gen_acc
+  `{M1 : LtsOba A L, !Good A L good, !gen_spec_acc co_of f} s O q :
   f O s ⟶ q ->
-  good q \/ (∃ μ s1 s2 s3, s = s1 ++ [μ] ++ s2 ++ [co μ] ++ s3
+  good q \/ (∃ μ s1 s2 s3, s = s1 ++ [μ] ++ s2 ++ [co_of μ] ++ s3
                           /\ q ⋍ f O (s1 ++ s2 ++ s3)
-                          /\ is_input μ /\ are_inputs s1 /\ are_inputs s2).
+                          /\ exist_co_nba μ
+                          /\ Forall exist_co_nba s1 
+                          /\ Forall exist_co_nba s2).
 Proof.
   intros.
   eapply inversion_gen_tau; eauto.
-  left. eapply gen_spec_acc_nil_stable_tau.
-  intro μ. right.
-  intros.  eapply gen_spec_acc_nil_lts_inp_good; eauto.
-Qed. *)
+  + left. eapply gen_spec_acc_nil_stable_tau.
+  + intro μ. destruct (decide (non_blocking μ)) as [nb | not_nb]. 
+    ++ left. eapply gen_spec_acc_nil_stable_nb. exact nb.
+    ++ right. intros μ' HypTr. eapply gen_spec_acc_nil_lts_not_nb_good.
+       +++ exact not_nb.
+       +++ exact HypTr. 
+Qed. 
 
 (** Converse implication of the first requirement. *)
 
@@ -656,39 +655,55 @@ Proof.
          (well_founded_induction (wf_inverse_image _ nat _ length Nat.lt_wf_0)).
   intros p hcnv.
   induction (cnv_terminate p s hcnv) as [p hp IHtp].
-  (* destruct (decide (good (gen_conv s))).
-  - eapply m_now; eauto.
-  -  *) apply m_step.
+  apply m_step.
   + eapply gen_spec_ungood.
   + edestruct gen_conv_always_reduces. eauto with mdb.
   + intros p' l. eapply IHtp; [|eapply cnv_preserved_by_lts_tau]; eauto.
   + intros e' l.
-    assert (good e') as happy.
-    eapply inversion_gen_tau_gen_conv; eauto.
-    eapply m_now; eauto.
+    destruct (inversion_gen_tau_gen_conv s e' l)
+      as [hu | (ν & s1 & s2 & s3 & eq__s & sc & i0 & i1 & i2)]; eauto with mdb.
+    eapply must_eq_client. symmetry. eassumption.
+    subst.
+    eapply Hlength.
+    ++ subst. rewrite 6 app_length. simpl. lia.
+    ++ inversion i0 (* as (x & nb & duo) *). destruct H3.
+       assert (x = co ν). eapply unique_nb; eauto. subst. 
+       eapply cnv_annhil; eauto. assert (co_of ν = co ν) as eq'.
+       eapply co_of_is_co_nb; eauto. rewrite eq' in hcnv. eauto. 
   + intros p' e' ν ν' inter hlp hle.
     destruct (inversion_gen_mu_gen_conv s ν' e' hle)
-      as [hg | (s1 & s2 & ν'' & heq & sc & eq & his)]; eauto with mdb. subst.
-    assert (ν'' = ν). eapply co_inter_spec1; eauto. subst.
-    eapply (cnv_drop_in_the_middle p s1 s2) in hlp; subst; eauto with mdb.
-    eapply must_eq_client. symmetry. eassumption.
-    eapply Hlength; subst; eauto with mdb.
-    rewrite 2 app_length. simpl. lia.
-(*     destruct s.
-    ++ exfalso. 
-       assert (gen_conv [] ↛[ν']) as stable.
-       eapply gen_spec_conv_nil_stable_mu.
-       assert (¬ gen_conv [] ↛[ν']) as not_stable.
-       eapply lts_stable_spec2; eauto. 
-       contradiction.
-    ++ assert (gen_conv (a :: s) ⟶[ν'] e') as hle'; eauto.
-       eapply gen_spec_out_lts_mu_uniq in hle' as (equiv' & eq'). subst.
+      as [hg | (s1 & s2 & ν'' & heq & sc & eq & his(*  & eq3 *))]; eauto with mdb.
+    rewrite heq in hle. subst. assert (ν'' = ν). eapply co_inter_spec1. eauto. subst.
+    
+    destruct (decide (non_blocking ν)) as [nb' | not_nb'].
+    ++ eapply (cnv_drop_non_blocking_action_in_the_middle p s1 s2) in hlp; subst; eauto with mdb.
        eapply must_eq_client. symmetry. eassumption.
        eapply Hlength; subst; eauto with mdb.
-       eapply co_inter_spec1 in inter. subst.
-       assert (p ⟹{ν} p') as weak_tr. eapply lts_to_wt; eauto.
-       eapply cnv_preserved_by_wt_act in hcnv; eauto. *)
-Qed.
+       rewrite 2 app_length. simpl. lia.
+    ++ destruct (decide (non_blocking (co_of ν))) as [nb | not_nb].
+       +++ eapply (cnv_drop_input_in_the_middle p s1 s2) in hlp; subst; eauto with mdb.
+           eapply must_eq_client. symmetry. eassumption.
+           eapply Hlength; subst; eauto with mdb.
+           rewrite 2 app_length. simpl. lia. esplit; eauto.
+       +++ destruct s1.
+            ++++ simpl in *.
+                 eapply must_eq_client. symmetry. eassumption.
+                 eapply Hlength; subst; eauto with mdb. eapply cnv_preserved_by_wt_act; eauto.
+                 eapply lts_to_wt;eauto.
+            ++++ inversion his as [|? ? Hyp]; subst. 
+                 destruct Hyp as (a' & nb' & duo').
+                 assert (a' = co a). eapply unique_nb; auto. 
+                 assert (co_of a = co a). eapply co_of_is_co_nb; eauto. 
+                 subst; eauto. subst; eauto.
+                 subst.
+                 assert (ν = a). admit. subst.
+                 assert (e' ⋍ gen_conv (s1 ++ a :: s2)). admit.
+                 eapply must_eq_client. symmetry. exact H4.
+                 eapply Hlength; auto.
+                 eapply (cnv_wt_prefix [a] (s1 ++ a :: s2) p).
+                 simpl. eauto.
+                 eapply lts_to_wt. auto. (* exfalso ? *)
+Admitted.
 
 Lemma must_iff_cnv `{
   @LtsObaFW P A H LtsP LtsEqP V,
@@ -714,13 +729,9 @@ Proof. intros hleq s hcnv. now eapply must_iff_cnv, hleq, must_iff_cnv. Qed.
 
 (** Second requirement for completeness *)
 
-Definition pre_acc_set_of `{Lts P A} (p : P) (μ : A) : Prop := ¬ lts_stable p (ActExt μ).
-
-Definition acc_set_of `{Lts P A} (p : P) : A -> Prop := pre_acc_set_of p.
-
 Definition oas `{FiniteImageLts P A} (p : P) (s : list A) (hcnv : p ⇓ s) : list (A -> Prop) :=
   let ps : list P := elements (wt_stable_set p s hcnv) in
-  (* ⋃  *) map acc_set_of ps.
+  (* ⋃  *) map lts_acc_set_of ps.
 
 Lemma exists_forall_in {B} (ps : list B) (P : B -> Prop) (Q : B -> Prop)
   (h : forall p, p ∈ ps -> P p \/ Q p) : Exists P ps \/ Forall Q ps.
@@ -739,8 +750,8 @@ Qed.
 Lemma wt_acceptance_set_subseteq
   `{FiniteImageLts P A} μ s p q hacnv1 hacnv2 :
   p ⟹{μ} q ->
-  map acc_set_of (elements (wt_stable_set q s hacnv1)) ⊆
-    map acc_set_of (elements (wt_stable_set p (μ :: s) hacnv2)).
+  map lts_acc_set_of (elements (wt_stable_set q s hacnv1)) ⊆
+    map lts_acc_set_of (elements (wt_stable_set p (μ :: s) hacnv2)).
 Proof.
   intros.
   intros a in__a.
@@ -755,8 +766,8 @@ Qed.
 
 Lemma lts_tau_acceptance_set_subseteq `{FiniteImageLts P A} s p q hacnv1 hacnv2 :
   p ⟶ q ->
-  map acc_set_of (elements $ wt_stable_set q s hacnv1) ⊆
-    map acc_set_of (elements $ wt_stable_set p s hacnv2).
+  map lts_acc_set_of (elements $ wt_stable_set q s hacnv1) ⊆
+    map lts_acc_set_of (elements $ wt_stable_set p s hacnv2).
 Proof.
   intros.
   intros a in__a.
@@ -795,210 +806,244 @@ Lemma aft_output_must_gen_acc `{
   `{@Prop_of_Inter P E A parallel_inter H LtsP LtsE}
 
   (p : P) μ s O :
-  p ⤓ -> (forall q, p ⟹{μ} q -> must q (gen_acc O s)) 
+  p ⤓ -> ¬ non_blocking (co_of μ) -> (forall q, p ⟹{μ} q -> must q (gen_acc O s)) 
               -> must p (gen_acc O (μ :: s) : E).
 Proof.
-  intros tp hmq. induction tp.
+  intro tp. (* not_nb hmq. *) revert O μ s. induction tp.
+  intros O μ s not_nb hmq.
   eapply m_step.
   - eapply gen_spec_ungood.
-  - edestruct (@gen_spec_out_lts_tau_ex E A); eauto with mdb.
+  - edestruct (@gen_spec_co_not_nb_lts_tau_ex E A); eauto with mdb. (* 3 *)
     now destruct gen_spec_acc0.
-  - intros. eapply H4. eassumption. intros.
+  - intros. eapply H4. eassumption. eassumption. 
     eauto with mdb.
   - intros e' l. eapply m_now.
-    apply (gen_spec_out_lts_tau_good μ s e'). eassumption.
+    apply (gen_spec_co_not_nb_lts_tau_good μ s e'). eassumption. eassumption.
   - intros p' e' μ' μ'' inter l0 l1.
-    eapply gen_spec_out_lts_mu_uniq in l1 as (h1 & h2). subst.
-    eapply must_eq_client. symmetry; eauto.
-    eapply hmq. eapply co_inter_spec1 in inter. subst. eauto with mdb.
-    
-    Unshelve. exact O.
+    eapply gen_spec_co_not_nb_lts_mu_uniq in l1 as (h1 & h2). subst.
+      eapply must_eq_client. symmetry; eauto.
+      eapply hmq. eapply co_inter_spec1 in inter. subst. eauto with mdb. eauto.
+    Unshelve. exact O. (* ?????? dû à (* 3 *)*)
 Qed.
 
-(* Lemma gen_acc_tau_ex
-  `{M1 : LtsObaFB A L, !Good A L good, !gen_spec_acc f} s1 s2 s3 μ O :
-  is_input μ -> are_inputs s1 -> are_inputs s2 ->
-  f O (s1 ++ [μ] ++ s2 ++ [co μ] ++ s3) ⟶⋍ f O (s1 ++ s2 ++ s3).
+Lemma gen_acc_tau_ex `{
+  M1 : LtsObaFB E A, !Good E A good, !gen_spec_acc co_of f} 
+  s1 s2 s3 μ O :
+  exist_co_nba μ -> Forall exist_co_nba s1 -> Forall exist_co_nba s2 ->
+  f O (s1 ++ [μ] ++ s2 ++ [co_of μ] ++ s3) ⟶⋍ f O (s1 ++ s2 ++ s3).
+  (* inversion_gen_tau *)
 Proof.
   intros.
-  assert (f O (s1 ++ [μ] ++ s2 ++ [co μ] ++ s3) ⟶⋍[co μ]
-            f O (s1 ++ s2 ++ [co μ] ++ s3)) as (e1 & l1 & heq1).
-  eapply (@f_gen_lts_mu_in_the_middle A L _ _ _ _ _ _ (f O) _
-            s1 (s2 ++ [co μ] ++ s3) μ); simpl in *; eauto.
-  assert (f O (s1 ++ s2 ++ [co μ] ++ s3) ⟶⋍[co (co μ)]
+  assert (f O (s1 ++ [μ] ++ s2 ++ [co_of μ] ++ s3) ⟶⋍[co_of μ]
+            f O (s1 ++ s2 ++ [co_of μ] ++ s3)) as (e1 & l1 & heq1).
+  eapply (@f_gen_lts_mu_in_the_middle E A _ _ _ _ _ _  co_of (f O) _
+            s1 (s2 ++ [co_of μ] ++ s3) μ); simpl in *; eauto. (* 3 *)
+  assert (f O (s1 ++ s2 ++ [co_of μ] ++ s3) ⟶⋍[co_of (co_of μ)]
             f O ((s1 ++ s2) ++ s3)) as (e2 & l2 & heq2).
-  replace (s1 ++ s2 ++ [co μ] ++ s3) with ((s1 ++ s2) ++ [co μ] ++ s3).
-  eapply (@f_gen_lts_mu_in_the_middle A L _ _ _ _ _ _ (f O) _
-            (s1 ++ s2) s3 (co μ)); simpl in *; eauto.
-  unfold are_inputs. eapply Forall_app; eauto.
+  replace (s1 ++ s2 ++ [co_of μ] ++ s3) with ((s1 ++ s2) ++ [co_of μ] ++ s3).
+  eapply (@f_gen_lts_mu_in_the_middle E A _ _ _ _ _ _ co_of (f O) _
+            (s1 ++ s2) s3 (co_of μ)); simpl in *; eauto. (* 3 *)
+  unfold exist_co_nba. eapply Forall_app; eauto.
   now rewrite <- app_assoc.
-  rewrite co_involution in l2.
-  destruct H2 as (a & eq). subst. simpl in *.
+  assert (μ =co_of (co_of μ)) as eq. eapply co_co_is_id.
+  rewrite <-eq in l2.
+  destruct H1 as (a' & nb & duo).
+  assert (a' = co μ). eapply unique_nb; eauto. subst.
+  assert (co_of μ = co μ) as eq'. eapply co_of_is_co_nb; eauto.
+  rewrite<- eq' in nb, duo.
+  (* subst.  *)simpl in *.
   edestruct (eq_spec e1 e2) as (e' & l' & heq'). eauto.
-  destruct (lts_oba_fb_feedback l1 l') as (t & lt & heqt); eauto.
+  destruct (lts_oba_fb_feedback nb duo l1 l') as (t & lt & heqt); eauto.
   exists t. split; eauto.
   rewrite <- app_assoc in heq2.
   transitivity e'. eauto.
   transitivity e2; eauto.
-Qed. *)
+  
+  Unshelve. eauto. eauto. (* ?????? dû à (* 3 *)*)
+Qed.
 
-(* Lemma must_f_gen_a_subseteq_non_blocking `{
-  @LtsObaFB E A H LtsE LtsEqE W, !Good E A good, !gen_spec_acc gen_acc} 
+Lemma must_f_gen_a_subseteq_non_blocking `{
+  @LtsObaFB E A H LtsE LtsEqE W, !Good E A good, !gen_spec_acc co_of gen_acc} 
   s e η O1 :
-  non_blocking η -> gen_acc O1 s ⟶[η] e -> forall O2, (forall μ, O1 μ -> O2 μ) 
+  non_blocking η -> gen_acc O1 s ⟶[η] e -> forall O2, O1 ⫅ O2 
     -> exists t, gen_acc O2 s ⟶[η] t.
 Proof.
   revert e O1.
   induction s as [|μ s']; intros e O1 nb l O2 hsub.
-  + exfalso. eapply lts_stable_spec2, gen_spec_acc_nil_stable_out. eauto. eauto.
+  + exfalso. eapply lts_stable_spec2, gen_spec_acc_nil_stable_nb. eauto. eauto.
   + destruct (decide (non_blocking μ)) as [nb' | not_nb'].
     ++ edestruct
-         (@gen_spec_mu_lts_co E A _ _ _ _ _ (gen_acc O2) _ μ s')
+         (@gen_spec_mu_lts_co E A _ _ _ _ _ co_of (gen_acc O2) _ μ s')
          as (r' & hl' & heqr').
-       edestruct (gen_spec_out_lts_mu_uniq l). subst. 
-       (* assert (parallel_inter μ (co_of μ)) as inter. eapply co_inter.
-       exfalso. *) admit.
+       assert (¬ non_blocking (co_of μ)) as not_nb. 
+       eapply lts_oba_fw_non_blocking_duo_spec; eauto. 
+       assert (parallel_inter (co_of μ) μ). symmetry. eapply co_inter. eauto.
+       edestruct (gen_spec_co_not_nb_lts_mu_uniq not_nb l). subst. contradiction. 
     ++ edestruct
-        (@gen_spec_mu_lts_co E A _ _ _ _ _ (gen_acc O1) _ μ s')
+        (@gen_spec_mu_lts_co E A _ _ _ _ _ co_of (gen_acc O1) _ μ s')
         as (e1 & hle1 & heqe1). (* simpl in hle1. *)
        edestruct
-         (@gen_spec_mu_lts_co E A _ _ _ _ _ (gen_acc O2) _ μ s')
+         (@gen_spec_mu_lts_co E A _ _ _ _ _ co_of (gen_acc O2) _ μ s')
          as (e2 & hle2 & heqe2). (* simpl in hle2. *)
-       destruct (decide (a = b)); subst; eauto.
-       assert (neq : ActOut a ≠ ActOut b) by now inversion 1.
-       destruct (lts_oba_output_confluence neq hle1 l) as
-         (r1 & l1 & r2 & l2 & heq).
-       edestruct (eq_spec (gen_acc O1 s') r1) as (e' & hle' & heqe').
-       symmetry in heqe1. eauto.
-       eapply IHs' in hle' as (t & hlt).
-       edestruct (eq_spec e2 t) as (e2' & hle2' & heqe2'). eauto.
-       edestruct (lts_oba_output_commutativity hle2 hle2') as (v & l3 & l4).
-       eauto with mdb. eassumption.
-Qed. *)
+       destruct (decide (non_blocking (co_of μ))) as [nb'' | not_nb''].
+       +++ destruct (decide (η = co_of μ)) as [eq | not_eq]. 
+           ++++ subst; eauto.
+           ++++ destruct (lts_oba_non_blocking_action_confluence nb'' not_eq hle1 l) as
+            (r1 & l1 & r2 & l2 & heq).
+           edestruct (eq_spec (gen_acc O1 s') r1) as (e' & hle' & heqe').
+           symmetry in heqe1. eauto.
+           eapply IHs' in hle' as (t & hlt); eauto.
+           edestruct (eq_spec e2 t) as (e2' & hle2' & heqe2'). eauto.
+           edestruct (lts_oba_non_blocking_action_delay nb'' hle2 hle2') as (v & l3 & l4).
+           eauto with mdb.
+       +++ assert (e ⋍ gen_acc O1 s' /\ η = co_of μ) as (equiv & eq).
+           eapply gen_spec_co_not_nb_lts_mu_uniq; eauto. subst.
+           exists e2. eauto.
+           Unshelve. eauto.
+Qed.
 
-Lemma must_f_gen_a_subseteq `{
+Lemma must_f_gen_a_subseteq_not_non_blocking `{
   @LtsObaFB E A H LtsE LtsEqE W, !Good E A good, !gen_spec_acc co_of gen_acc} 
-  s e μ O1 :
-  gen_acc O1 s ⟶[μ] e -> forall O2, (forall μ, O1 μ -> O2 μ) -> exists t, gen_acc O2 s ⟶[μ] t.
+  s e μ' O1 :
+  ¬ non_blocking μ' -> gen_acc O1 s ⟶[μ'] e -> forall O2, O1 ⫅ O2 
+      -> exists t, gen_acc O2 s ⟶[μ'] t.
 Proof.
   revert e O1.
-  induction s as [|μ' s']; intros e O1 l O2 hsub.
-  + destruct (decide (non_blocking μ)) as [nb | not_nb].
-    ++ rename μ into η. exfalso.
-       eapply lts_stable_spec2, gen_spec_acc_nil_stable_out. eauto. eauto.
-    ++ eapply gen_spec_acc_nil_mu_inv in not_nb as (μ' & inter & mem); eauto.
-       eapply hsub in mem. 
-       eapply gen_spec_acc_nil_mem_lts_inp in mem as (t & μ'' & HypTr & eq).
-       subst. exists t. eauto.
-  + edestruct
-        (@gen_spec_mu_lts_co E A _ _ _ _ _ co_of (gen_acc O1) _ μ' s')
-        as (e1 & hle1 & heqe1).
-    edestruct
-         (@gen_spec_mu_lts_co E A _ _ _ _ _ co_of (gen_acc O2) _ μ' s')
-         as (e2 & hle2 & heqe2).
-    eapply 
-  
-  
-  eapply gen_spec_out_lts_mu_uniq in l as (equiv & eq). subst.
-    exists (gen_acc O2 s').
-    apply gen_spec_mu_lts_co.
-    
-  
-  assert (exists e,  gen_acc O2 (μ' :: s') ⟶[μ] e -> e ⋍ gen_acc O2 s' /\ μ = co_of μ') as sol.
-    eexists. eapply gen_spec_out_lts_mu_uniq.
-    destruct sol as (e' & Hyp).
-    exists e'. eauto.
-    
-    
-  
-    destruct μ as [b|b].
+  induction s as [|μ s']; intros e O1 not_nb l O2 hsub.
+  + eapply gen_spec_acc_nil_mu_inv in l as (μ'' & eq & In) ; eauto. subst.
+    eapply hsub in In.
+    eapply gen_spec_acc_nil_mem_lts_inp in In as (r & μ''' & HypTr & eq). subst.
+    eauto.
+  + destruct (decide (non_blocking (co_of μ))) as [nb' | not_nb'].
     ++ edestruct
-        (@gen_spec_mu_lts_co B L _ _ _ _ _ (gen_acc O1) _ (ActIn b) s')
-        as (r & hl & heqr). simpl in hl.
-       assert (neq : ActIn a ≠ ActOut b) by now inversion 1.
-       destruct (lts_oba_output_confluence neq hl l) as
+        (@gen_spec_mu_lts_co E A _ _ _ _ _ co_of (gen_acc O1) _ μ s')
+        as (r & hl & heqr). (* simpl in hl. *)
+       assert (not_eq :  μ' ≠ (co_of μ)). intro impossible. subst. contradiction.
+       destruct (lts_oba_non_blocking_action_confluence nb' not_eq hl l) as
          (r1 & l1 & r2 & l2 & heq).
        edestruct (eq_spec (gen_acc O1 s') r1) as (e' & hle' & heqe').
        symmetry in heqr. eauto.
        eapply IHs' in hle' as (t & hlt).
        edestruct
-         (@gen_spec_mu_lts_co B L _ _ _ _ _ (gen_acc O2) _ (ActIn b) s')
+         (@gen_spec_mu_lts_co E A _ _ _ _ _ co_of (gen_acc O2) _ μ s')
          as (r' & hl' & heqr'). simpl in hl'.
        edestruct (eq_spec r' t) as (e2 & hle2 & heqe2). eauto.
-       edestruct (lts_oba_output_commutativity hl' hle2) as (v & l3 & l4).
-       eauto with mdb. eassumption.
+       edestruct (lts_oba_non_blocking_action_delay nb' hl' hle2) as (v & l3 & l4).
+       eauto with mdb. eassumption. eauto.
     ++ edestruct
-         (@gen_spec_mu_lts_co B L _ _ _ _ _ (gen_acc O2) _ (ActOut b) s')
+         (@gen_spec_mu_lts_co E A _ _ _ _ _ co_of (gen_acc O2) _ μ s')
          as (r' & hl' & heqr').
-       edestruct (gen_spec_out_lts_mu_uniq l); eauto. subst.
-       assert (a = b) by now inversion H1. subst. eauto.
+       edestruct (gen_spec_co_not_nb_lts_mu_uniq not_nb' l); eauto. subst. eauto.
 Qed.
 
-Lemma must_f_gen_a_subseteq_tau
-  `{@LtsObaFB B L IL LB LOB W, !Good B L good, !gen_spec_acc gen_acc}
-  s e O1 : gen_acc O1 s ⟶ e -> forall O2, O1 ⊆ O2 -> exists t, gen_acc O2 s ⟶ t.
+Lemma must_f_gen_a_subseteq_tau `{
+  @LtsObaFB E A H LtsE LtsEqE W, !Good E A good, !gen_spec_acc co_of gen_acc}
+  s e O1 : gen_acc O1 s ⟶ e -> forall O2, (forall μ, O1 μ -> O2 μ) 
+      -> exists t, gen_acc O2 s ⟶ t.
 Proof.
   revert e O1.
   induction s as [|μ s']; intros e O1 l O2 hsub.
   + exfalso. eapply lts_stable_spec2, gen_spec_acc_nil_stable_tau; eauto.
-  + destruct μ as [a|a].
+  + destruct (decide (non_blocking (co_of μ))) as [nb | not_nb].
     ++ edestruct
-        (@gen_spec_mu_lts_co B L _ _ _ _ _ (gen_acc O1) _ (ActIn a) s')
-        as (r & hl & heqr). simpl in hl.
-       destruct (lts_oba_output_tau hl l) as [(r1 & l1 & (r2 & l2 & heq))|].
+        (@gen_spec_mu_lts_co E A _ _ _ _ _ co_of (gen_acc O1) _ μ s')
+        as (r & hl & heqr). (* simpl in hl. *)
+       destruct (lts_oba_non_blocking_action_tau nb hl l) 
+        as [(r1 & l1 & (r2 & l2 & heq))| (μ' & duo & (r' & hl' & heq'))].
        +++ edestruct (eq_spec (gen_acc O1 s') r1) as (e' & hle' & heqe').
            symmetry in heqr. eauto.
            eapply IHs' in hle' as (t & hlt).
            edestruct
-             (@gen_spec_mu_lts_co B L _ _ _ _ _ (gen_acc O2) _ (ActIn a) s')
+             (@gen_spec_mu_lts_co E A _ _ _ _ _ co_of (gen_acc O2) _ μ s')
              as (r' & hl' & heqr'). simpl in hl'.
            edestruct (eq_spec r' t) as (e2 & hle2 & heqe2). eauto.
-           edestruct (lts_oba_output_commutativity hl' hle2) as (v & l3 & l4).
+           edestruct (lts_oba_non_blocking_action_delay nb hl' hle2) as (v & l3 & l4).
            eauto with mdb. eassumption.
-       +++ edestruct H0 as (r' & hl' & heq').
-           edestruct (eq_spec (gen_acc O1 s') r') as (t & hlt & heqt).
+       +++ edestruct (eq_spec (gen_acc O1 s') r') as (t & hlt & heqt).
            symmetry in heqr. eauto.
-           edestruct (must_f_gen_a_subseteq_input s' t a O1 hlt O2 hsub).
+           assert (¬ non_blocking μ') as not_nb. 
+           eapply lts_oba_fw_non_blocking_duo_spec; eauto.
+           edestruct (must_f_gen_a_subseteq_not_non_blocking s' t μ' O1 not_nb hlt O2 hsub).
            edestruct
-             (@gen_spec_mu_lts_co B L _ _ _ _ _ (gen_acc O2) _ (ActIn a) s')
+             (@gen_spec_mu_lts_co E A _ _ _ _ _ co_of (gen_acc O2) _ μ' s')
              as (u & hlu & hequ).
            edestruct (eq_spec u x) as (t' & hlt' & heqt'). eauto.
-           edestruct (lts_oba_fb_feedback hlu hlt'); eauto.
+           assert (μ = μ'). eapply co_inter_spec1. eauto. subst.
+           edestruct (lts_oba_fb_feedback nb duo hlu hlt'); eauto.
            firstorder.
-    ++ eapply gen_spec_out_lts_tau_ex.
+    ++ eapply gen_spec_co_not_nb_lts_tau_ex. exact not_nb.
+    
+    Unshelve. eauto.
 Qed.
 
-Lemma must_f_gen_a_subseteq_nil
-  `{@Lts A L IL, @LtsObaFB B L IL LB LOB W, !Good B L good, !gen_spec_acc gen_acc}
-  (p : A) O1 : must p (gen_acc O1 []) -> forall O2, O1 ⊆ O2 -> must p (gen_acc O2 []).
+Lemma must_f_gen_a_subseteq_nil `{
+  LtsP : @Lts P A H, 
+  @LtsObaFB E A H LtsE LtsEqE W, !Good E A good, !gen_spec_acc co_of gen_acc}
+
+  `{@Prop_of_Inter P E A parallel_inter H LtsP LtsE}
+
+  (p : P) O1 : 
+  must p (gen_acc O1 []) -> forall O2, O1 ⫅ O2 -> must p (gen_acc O2 []).
 Proof.
   intros hm.
   assert (hpt : p ⤓)
     by now (eapply must_terminate_ungood, gen_spec_ungood; eauto).
   induction hpt. dependent induction hm; intros O2 hsub.
-  - now eapply gen_spec_ungood in H1.
+  - now eapply gen_spec_ungood in H2.
   - eapply m_step; eauto with mdb.
     + eapply gen_spec_ungood.
     + destruct ex as ((p' & e') & l').
       inversion l'; subst.
       +++ eauto with mdb.
-      +++ exfalso. eapply lts_stable_spec2, gen_spec_acc_nil_stable_tau; eauto.
-      +++ destruct α1 as [[b|b]|]; destruct α2 as [[a|a]|]; inversion eq; subst.
-          exfalso. eapply lts_stable_spec2, gen_spec_acc_nil_stable_out; eauto.
-          eapply gen_spec_acc_nil_mu_inv, hsub, gen_spec_acc_nil_mem_lts_inp
-            in l2 as (e & l).
-          eauto with mdb.
+      +++ exfalso. assert ({q : E | gen_acc O1 [] ⟶ q}) as impossible.
+          eauto.
+          eapply lts_stable_spec2 in impossible. 
+          assert (gen_acc O1 [] ↛). eapply gen_spec_acc_nil_stable_tau ; eauto.
+          contradiction.
+      +++ destruct (decide (non_blocking μ1)) as [nb1 | not_nb1]; 
+          destruct (decide (non_blocking μ2)) as [nb2 | not_nb2].
+          ++++ contradict nb1.
+               eapply lts_oba_fw_non_blocking_duo_spec; eauto.
+          ++++ eapply gen_spec_acc_nil_mu_inv in l2 as (μ & eq' & In). subst.
+               eapply hsub in In.
+               apply gen_spec_acc_nil_mem_lts_inp in In as (e & μ' & l & eq'). subst.
+               eauto with mdb. eauto with mdb.
+          ++++ exfalso.
+               assert ({q : E | gen_acc O1 [] ⟶[μ2] q}) as impossible. eauto.
+               eapply lts_stable_spec2 in impossible. 
+               assert (gen_acc O1 [] ↛[μ2]). eapply gen_spec_acc_nil_stable_nb ; eauto.
+               contradiction.
+          ++++ eapply gen_spec_acc_nil_mu_inv in l2 as (μ & eq' & In). subst.
+               eapply hsub in In.
+               apply gen_spec_acc_nil_mem_lts_inp in In as (e & μ' & l & eq'). subst.
+               eauto with mdb. eauto with mdb.
     + intros e l.
-      exfalso. eapply lts_stable_spec2, gen_spec_acc_nil_stable_tau; eauto.
-    + intros p' e' μ l1 l2.
-      eapply gen_spec_acc_nil_lts_inp_good in l1. eauto with mdb.
+      exfalso. 
+      assert ({q : E | gen_acc O2 [] ⟶ q}) as impossible. eauto.
+      eapply lts_stable_spec2 in impossible. 
+      assert (gen_acc O2 [] ↛). eapply gen_spec_acc_nil_stable_tau ; eauto.
+      contradiction.
+    + intros p' e' μ μ' inter l2 l1.
+      destruct (decide (non_blocking μ')) as [nb | not_nb].
+      ++ exfalso. 
+         assert ({q : E | gen_acc O2 [] ⟶[μ'] q}) as impossible. eauto.
+         eapply lts_stable_spec2 in impossible. 
+         assert (gen_acc O2 [] ↛[μ']). eapply gen_spec_acc_nil_stable_nb ; eauto.
+         contradiction.
+      ++ eapply gen_spec_acc_nil_lts_not_nb_good in l1. eauto with mdb. eauto.
 Qed.
 
-Lemma must_f_gen_a_subseteq
-  `{@Lts A L IL,
-    @LtsObaFB B L IL LB LOB W, !Good B L good,
-    !gen_spec_acc gen_acc} s (p : A) O1 :
-  must p (gen_acc O1 s) -> forall O2, O1 ⊆ O2 -> must p (gen_acc O2 s).
+Lemma must_f_gen_a_subseteq `{
+  LtsP : @Lts P A H,
+  @LtsObaFB E A H LtsE LtsEqE W, !Good E A good,
+    !gen_spec_acc co_of gen_acc}
+
+  `{@Prop_of_Inter P E A parallel_inter H LtsP LtsE}
+
+  s (p : P) O1 :
+  
+  must p (gen_acc O1 s) -> forall O2, O1 ⫅ O2
+      -> must p (gen_acc O2 s).
 Proof.
   revert p O1.
   induction s
@@ -1008,42 +1053,59 @@ Proof.
   - eapply must_f_gen_a_subseteq_nil; eauto.
   - assert (htp : p ⤓) by (eapply must_terminate_ungood, gen_spec_ungood; eauto).
     induction htp.
-    inversion hm. now eapply gen_spec_ungood in H3.
+    inversion hm. now eapply gen_spec_ungood in H4.
     eapply m_step; eauto with mdb.
     + eapply gen_spec_ungood.
     + destruct ex as (t & l). inversion l; subst; eauto with mdb.
       ++ eapply must_f_gen_a_subseteq_tau in l0 as (e & hle); eauto with mdb.
-      ++ destruct α1 as [[b|b]|]; destruct α2 as [[a|a]|]; inversion eq; subst.
-         eapply must_f_gen_a_subseteq_output in l2 as (t & hl); eauto with mdb.
-         eapply must_f_gen_a_subseteq_input in l2 as (t & hl); eauto with mdb.
+      ++ destruct (decide (non_blocking μ1)) as [nb1 | not_nb1]; 
+         destruct (decide (non_blocking μ2)) as [nb2 | not_nb2].
+         +++ contradict nb1. 
+             eapply lts_oba_fw_non_blocking_duo_spec; eauto.
+         +++ eapply must_f_gen_a_subseteq_not_non_blocking in l2 as (t & hl); eauto with mdb.
+         +++ eapply must_f_gen_a_subseteq_non_blocking in l2 as (t & hl); eauto with mdb.
+         +++ eapply must_f_gen_a_subseteq_not_non_blocking in l2 as (t & hl); eauto with mdb.
     + intros e' l.
-      edestruct inversion_gen_tau_gen_acc as [|H3]; eauto with mdb.
-      destruct H3 as (μ & s1 & s2 & s3 & heqs & sc & himu & his1 & his2).
+      edestruct inversion_gen_tau_gen_acc as [|Hyp]; eauto with mdb.
+      destruct Hyp as (μ & s1 & s2 & s3 & heqs & sc & himu & his1 & his2).
       eapply (must_eq_client p (gen_acc O2 (s1 ++ s2 ++ s3))). now symmetry.
       edestruct (gen_acc_tau_ex s1 s2 s3 μ O1) as (t & hlt & heqt); eauto.
       eapply Hlength; eauto.
       ++ rewrite heqs, 6 app_length. simpl. lia.
       ++ eapply must_eq_client. eapply heqt. eapply et. now rewrite heqs.
-    + intros p' e' μ l1 l2.
-      edestruct inversion_gen_mu_gen_acc as [|H3]; eauto with mdb.
-      destruct H3 as (s1 & s2 & heqs & heq & his1).
+    + intros p' e' μ μ' inter l1 l2.
+      edestruct inversion_gen_mu_gen_acc as [|Hyp]; eauto with mdb.
+      destruct Hyp as (s1 & s2 & μ''' & heqs & heq & eq & his1). subst.
       eapply must_eq_client. symmetry. eassumption.
       edestruct @f_gen_lts_mu_in_the_middle as (t & l & heq'); eauto.
       now destruct gen_spec_acc0.
       eapply Hlength. rewrite heqs.
       rewrite 2 app_length. simpl. lia.
       eapply must_eq_client. eapply heq'.
-      eapply com. rewrite heqs. eassumption.
-      now rewrite co_involution. eassumption.
+      eapply com; eauto. rewrite heqs. eassumption.
+      eassumption.
 Qed.
 
-Lemma must_gen_acc_stable
-  `{@LtsOba A L IL LA LOA, @LtsOba B L IL LB LOB, !Good B L good, !gen_spec_acc gen_acc}
-  (p : A) O : p ↛ -> must p (gen_acc (lts_outputs p ∖ O) []) \/ lts_outputs p ⊆ O.
+
+
+Lemma must_gen_acc_stable `{
+  @LtsOba P A H LtsP LtsEqP, 
+  @LtsOba E A H LtsE LtsEqE, !Good E A good, !gen_spec_acc co_of gen_acc}
+
+  `{@Prop_of_Inter P E A parallel_inter H LtsP LtsE}
+
+  (p : P) O : 
+
+  p ↛ -> must p (gen_acc (lts_acc_set_of p \ O) []) 
+         \/ lts_acc_set_of p ⫅ O.
 Proof.
   intros.
-  remember (lts_outputs p ∖ O) as D.
-  destruct D as [|a D'] using set_ind_L.
+  remember (lts_acc_set_of p \ O ) as D. 
+  
+  (*définir l'inductivité sur les prédicat *)
+  
+  
+(*   destruct D as [|a D'] using set_ind_L.
   + right. set_solver.
   + left.
     eapply m_step.
@@ -1060,20 +1122,24 @@ Proof.
        eapply gen_spec_acc_nil_stable_tau.
     ++ intros p' e' μ l0 l1.
        destruct μ.
-       eapply gen_spec_acc_nil_lts_inp_good in l0. eauto with mdb.
+       eapply gen_spec_acc_nil_lts_not_nb_good in l0. eauto with mdb.
        exfalso.
        eapply (@lts_stable_spec2 B); eauto with mdb.
-       eapply gen_spec_acc_nil_stable_out.
-Qed.
+       eapply gen_spec_acc_nil_stable_nb. *)
+Admitted.
 
-Lemma must_gen_a_with_nil
-  `{@LtsObaFW A L IL LA LOA V, @LtsObaFB B L IL LB LOB W,
-    !FiniteLts A L, !Good B L good,
-    !gen_spec_acc gen_acc} (p : A) (hcnv : p ⇓ []) O :
-  (exists p', p ⟹ p' /\ lts_stable p' τ /\ lts_outputs p' ⊆ O)
-  \/ must p (gen_acc (oas p [] hcnv ∖ O) []).
+Lemma must_gen_a_with_nil `{
+  @LtsObaFW P A H LtsP LtsEqP V, !FiniteImageLts P A,
+  @LtsObaFB E A H LtsE LtsEqE W, !Good E A good, !gen_spec_acc co_of gen_acc}
+
+  `{@Prop_of_Inter P E A parallel_inter H LtsP LtsE}
+
+  (p : P) (hcnv : p ⇓ []) O :
+
+  (exists p', p ⟹ p' /\ lts_stable p' τ /\ lts_acc_set_of p' ⫅ O).
+  (* \/ must p (gen_acc (oas p [] hcnv \ O) []). *)
 Proof.
-  induction (cnv_terminate p [] hcnv) as (p, hpt, ihhp).
+(*   induction (cnv_terminate p [] hcnv) as (p, hpt, ihhp).
   destruct (decide (lts_stable p τ)) as [st | (p' & l)%lts_stable_spec1].
   - destruct (must_gen_acc_stable p O st).
     + right. unfold oas.
@@ -1102,15 +1168,21 @@ Proof.
          now eapply lts_tau_set_spec. eassumption.
       ++ intros e' l'. exfalso.
          eapply (@lts_stable_spec2 B). eauto. eapply gen_spec_acc_nil_stable_tau.
-      ++ intros p0 e0 μ le%gen_spec_acc_nil_lts_inp_good lp; eauto with mdb.
-Qed.
+      ++ intros p0 e0 μ le%gen_spec_acc_nil_lts_not_nb_good lp; eauto with mdb. *)
+Admitted.
 
-Lemma must_gen_a_with_s
-  `{@LtsObaFW A L IL LA LOA V, @LtsObaFB B L IL LB LOB W,
-    !FiniteLts A L, !Good B L good, !gen_spec_acc gen_acc} s (p : A) (hcnv : p ⇓ s) O :
-  (exists p', p ⟹[s] p' /\ lts_stable p' τ /\ lts_outputs p' ⊆ O) \/ must p (gen_acc (oas p s hcnv ∖ O) s).
+Lemma must_gen_a_with_s `{
+  @LtsObaFW P A H LtsP LtsEqP V, !FiniteImageLts P A,
+  @LtsObaFB E A H LtsE LtsEqE W, !Good E A good, !gen_spec_acc co_of gen_acc} 
+
+  `{@Prop_of_Inter P E A parallel_inter H LtsP LtsE}
+
+  s (p : P) (hcnv : p ⇓ s) O :
+
+  (exists p', p ⟹[s] p' /\ lts_stable p' τ /\ lts_acc_set_of p' ⫅ O).
+        (* \/ must p (gen_acc (oas p s hcnv ∖ O) s). *)
 Proof.
-  revert p hcnv O.
+(*   revert p hcnv O.
   induction s as [|μ s'].
   - eapply must_gen_a_with_nil.
   - intros p hcnv O.
@@ -1138,62 +1210,111 @@ Proof.
          eapply (must_eq_client _ _ _ (symmetry heqe')).
          edestruct (H1 p') as (? & hm).
          eapply wt_set_mu_spec2; eauto with mdb.
-         eapply must_f_gen_a_subseteq, difference_mono_r, union_wt_outputs_subseteq; eauto with mdb.
+         eapply must_f_gen_a_subseteq, difference_mono_r, 
+          union_wt_outputs_subseteq; eauto with mdb.
       ++ eapply aft_output_must_gen_acc; eauto.
          intros p' hw. edestruct (H1 p') as (? & hm).
          eapply wt_set_mu_spec2; eauto.
-         eapply must_f_gen_a_subseteq, difference_mono_r, union_wt_outputs_subseteq; eauto with mdb.
-Qed.
+         eapply must_f_gen_a_subseteq, difference_mono_r, 
+          union_wt_outputs_subseteq; eauto with mdb. *)
+Admitted.
 
-Lemma not_must_gen_a_without_required_output
-  `{@LtsObaFW A L IL LA LOA V, @LtsObaFB B L IL LB LOB W,
-    !Good B L good, !gen_spec_acc gen_acc} (q q' : A) s O :
-  q ⟹[s] q' -> q' ↛ -> ¬ must q (gen_acc (O ∖ lts_outputs q') s).
+Lemma not_must_gen_a_without_required_acc_set `{
+  @LtsObaFW P A H LtsP LtsEqP V, 
+  @LtsObaFB E A H LtsE LtsEqE W, !Good E A good, !gen_spec_acc co_of gen_acc} 
+
+  `{@Prop_of_Inter P E A parallel_inter H LtsP LtsE}
+
+  (q q' : P) s O :
+
+  q ⟹[s] q' -> q' ↛ -> ¬ must q (gen_acc (O \ lts_acc_set_of q') s).
 Proof.
   intros wt hst.
   dependent induction wt; intros hm.
-  - inversion hm; subst.
-    ++ contradict H1. eapply gen_spec_ungood.
+  - inversion hm as [happy | ]; subst.
+    ++ contradict happy. eapply gen_spec_ungood.
     ++ destruct ex as (t & l). inversion l; subst.
        +++ eapply (lts_stable_spec2 p τ); eauto with mdb.
        +++ exfalso. eapply lts_stable_spec2, gen_spec_acc_nil_stable_tau; eauto.
-       +++ destruct α1 as [[b|b]|]; destruct α2 as [[a|a]|]; inversion eq; subst.
-           eapply lts_stable_spec2, gen_spec_acc_nil_stable_out; eauto.
-           eapply gen_spec_acc_nil_mu_inv in l2.
-           eapply lts_outputs_spec1 in l1. set_solver.
+       +++ destruct (decide (non_blocking μ1)) as [nb1 | not_nb1]; 
+           destruct (decide (non_blocking μ2)) as [nb2 | not_nb2].
+           ++++ contradict nb1. 
+                eapply lts_oba_fw_non_blocking_duo_spec; eauto.
+           ++++ eapply gen_spec_acc_nil_mu_inv in l2 as (μ' & eq' & In); eauto. subst.
+                assert (μ' = μ1). eapply co_inter_spec1. eassumption. subst.
+                assert (lts_acc_set_of p μ1) as not_stable.
+                assert ({p' : P | p ⟶[μ1] p'}) as Hyp. eauto. 
+                eapply lts_stable_spec2 in Hyp.
+                intro stable. contradiction.
+                destruct In.
+                contradiction.
+           ++++ eapply lts_stable_spec2, gen_spec_acc_nil_stable_nb; eauto.
+           ++++ eapply gen_spec_acc_nil_mu_inv in l2 as (μ' & eq' & In); eauto. subst.
+                assert (μ' = μ1). eapply co_inter_spec1. eassumption. subst.
+                assert (lts_acc_set_of p μ1) as not_stable.
+                assert ({p' : P | p ⟶[μ1] p'}) as Hyp. eauto. 
+                eapply lts_stable_spec2 in Hyp.
+                intro stable. contradiction.
+                destruct In.
+                contradiction.
   - eapply (IHwt hst), (must_preserved_by_lts_tau_srv p q _ hm l).
   - eapply (IHwt hst).
-    assert (gen_acc (O ∖ lts_outputs t) (μ :: s) ⟶⋍[co μ]
-              gen_acc (O ∖ lts_outputs t) s) as (e' & hle' & heqe').
+    assert (gen_acc (O \ lts_acc_set_of t) (μ :: s) ⟶⋍[co_of μ]
+              gen_acc (O \ lts_acc_set_of t) s) as (e' & hle' & heqe')
     by eapply gen_spec_mu_lts_co.
     eapply must_eq_client; eauto.
-    inversion hm; subst. now eapply gen_spec_ungood in H1. destruct μ; eauto.
+    inversion hm as [happy |]; subst.
+    + now eapply gen_spec_ungood in happy.
+    + assert (parallel_inter μ (co_of μ)) as inter. eapply co_inter. eauto.
+    
+    Unshelve. eauto. eauto. eauto.
 Qed.
 
-Lemma completeness2
-  `{@LtsObaFW A L IL LA LOA V, @LtsObaFB B L IL LB LOB W,
-    @LtsObaFW C L IL LC LOC VC,
-    !FiniteLts A L, !FiniteLts C L, !Good B L good, !gen_spec_acc gen_acc}
-  (p : A) (q : C) : p ⊑ q -> p ≼₂ q.
+Lemma completeness2 `{
+  @LtsObaFW P A H LtsP LtsEqP VP, !FiniteImageLts P A,
+  @LtsObaFW Q A H LtsQ LtsEqQ VQ, !FiniteImageLts Q A,
+  @LtsObaFB E A H LtsE LtsEqE W, !Good E A good, !gen_spec_acc co_of gen_acc}
+
+  `{@Prop_of_Inter P E A parallel_inter H LtsP LtsE}
+  `{@Prop_of_Inter Q E A parallel_inter H LtsQ LtsE}
+
+  (p : P) (q : Q) : p ⊑ q -> p ≼₂ q.
 Proof.
   intros hpre s q' hacnv w st.
-  destruct (must_gen_a_with_s s p hacnv (lts_outputs q')) as [|hm] ; eauto.
-  eapply hpre in hm. contradict hm.
-  eapply not_must_gen_a_without_required_output; set_solver.
+  destruct (must_gen_a_with_s s p hacnv (lts_acc_set_of q')) (*as  [|hm] *).
+  + eauto.
+  (* + eapply hpre in hm. contradict hm.
+    eapply not_must_gen_a_without_required_output; set_solver. *)
 Qed.
 
-Lemma completeness_fw
-  `{@LtsObaFW A L IL LA LOA V, @LtsObaFW B L IL LB LOB W, @LtsObaFB C L IL LC LOC VC,
-    !FiniteLts A L, !FiniteLts B L, !FiniteLts C L, !Good C L good,
-    !gen_spec_conv gen_conv, !gen_spec_acc gen_acc}
-  (p : A) (q : B) : p ⊑ q -> p ≼ q.
+Lemma completeness_fw `{
+  @LtsObaFW P A H LtsP LtsEqP VP, !FiniteImageLts P A,
+  @LtsObaFW Q A H LtsQ LtsEqQ VQ, !FiniteImageLts Q A, 
+  @LtsObaFB E A H LtsE LtsEqE VC, !FiniteImageLts E A, !Good E A good,
+  !gen_spec_conv co_of gen_conv, !gen_spec_acc co_f gen_acc}
+
+  `{@Prop_of_Inter P E A parallel_inter H LtsP LtsE}
+  `{@Prop_of_Inter Q E A parallel_inter H LtsQ LtsE}
+
+  (p : P) (q : Q) : p ⊑ q -> p ≼ q.
 Proof. intros. split. now apply completeness1. now apply completeness2. Qed.
 
-Lemma completeness
-  `{@LtsObaFB A L IL LA LOA V, @LtsObaFB B L IL LB LOB W, @LtsObaFB C L IL LC LOC VC,
-    !FiniteLts A L, !FiniteLts B L, !FiniteLts C L, !Good C L good,
-    !gen_spec_conv gen_conv, !gen_spec_acc gen_acc}
-  (p : A) (q : B) : p ⊑ q -> p ▷ ∅ ≼ q ▷ ∅.
+Lemma completeness `{
+  @LtsObaFB P A H LtsP LtsEqP VP, !FiniteImageLts P A,
+  @LtsObaFB Q A H LtsQ LtsEqQ VQ, !FiniteImageLts Q A,
+  @LtsObaFB E A H LtsE LtsEqE VE, !FiniteImageLts E A, !Good E A good,
+  !gen_spec_conv co_of gen_conv, !gen_spec_acc co_of gen_acc}
+
+  `{@Prop_of_Inter P E A parallel_inter H LtsP LtsE}
+  `{@Prop_of_Inter Q E A parallel_inter H LtsQ LtsE}
+
+  `{@Prop_of_Inter P (mb A) A fw_inter H LtsP MbLts}
+  `{@Prop_of_Inter (P * mb A) E A parallel_inter H (inter_lts fw_inter) LtsE}
+
+  `{@Prop_of_Inter Q (mb A) A fw_inter H LtsQ MbLts}
+  `{@Prop_of_Inter (Q * mb A) E A parallel_inter H (inter_lts fw_inter) LtsE}
+
+  (p : P) (q : Q) : p ⊑ q -> p ▷ ∅ ≼ q ▷ ∅.
 Proof.
   intros hctx.
   eapply completeness_fw.
